B-unification/lowenheim.v
@@ -1,5 +1,6 @@
 (*
   Lowenheim's Formula
+
   Authors:
     Joseph St. Pierre
     Spyridon Antonatos
@@ -8,3 +9,29 @@
 (* Required Libraries *)
 
 Require Export terms.
+
+Require Import List.
+Import ListNotations.
+
+
+(** LOWENHEIM'S FORMULA **)
+
+(* Maps boolean number to term *)
+Definition tau (b : bool) : term :=
+  match b with
+    | false => T0
+    | true  => T1
+  end.
+
+(* Creates a single replacement (var -> term) for lowenheim's formula *)
+Definition lowenheim_replace (t : term) (v : var) (b : bool) : replacement :=
+  if (term_contains_var t v) then (v, (t + T1) * VAR v + t * (tau b))
+  else (v, VAR v).
+
+(* Creates a substitution (list replacement) for lowenheim's formula. Any variables entered into vars will be 
+   set to 1 *)
+Fixpoint lowenheim_subst (t : term) (term_vars : var_set) (vars : var_set) : subst :=
+  match term_vars with (* Ensure term_vars is unique *)
+    | nil => nil (* Can't create a substitution for a term with no variables! *)
+    | v :: v' => (lowenheim_replace t v (var_set_includes_var v vars)) :: (lowenheim_subst t v' vars)
+  end.
